tests/lean/run/smt_assert_define.lean
@@ -1,14 +1,14 @@
 open smt_tactic
 
+constant p : nat → nat → Prop
+constant f : nat → nat
+axiom pf (a : nat) : p (f a) (f a) → p a a
+
 example (a b c : nat) : a = b + 0 → a + c = b + c :=
 by using_smt $ do
   pr ← tactic.to_expr `(add_zero b),
   note `h pr,
   trace_state, return ()
-
-constant p : nat → nat → Prop
-constant f : nat → nat
-axiom pf (a : nat) : p (f a) (f a) → p a a
 
 example (a b c : nat) : a = b → p (f a) (f b) → p a b :=
 by using_smt $ do
@@ -20,3 +20,14 @@ by using_smt $ do
   note `h2 pr,
   trace_state,
   return ()
+
+example (a b c : nat) : a = b + 0 → a + c = b + c :=
+begin [smt]
+  add_fact add_zero b
+end
+
+example (a b c : nat) : a = b → p (f a) (f b) → p a b :=
+begin [smt]
+  assert h : p (f a) (f a),
+  add_fact (pf _ h)
+end
